Advection Equation

\partial u / \partial t = a \partial u / \partial x

Forward Scheme

u(t + dt, x) = u(t,x) + a dt/dx ( u(t,x) - u(t,x-dx) )

Stability

Condition:

G = | u(t+dt,x) / u(t,x) | < 1

Ansatz:

u(t,x) = c \exp(\alpha t + i \beta x)
G =  c \exp(\alpha (t + dt) + i \beta x) / c \exp(\alpha t + i \beta x) = \exp(\alpha dt)


e^{a dt} = 1 + a dt/dx ( 1 - e^{ - i \beta dx} )
e^{a dt} = 1 + a dt/dx ( 1 - \cos( \beta dx) + i \sin(\beta dx) )
|G| = (  1 + a dt/dx ( 1 - \cos( \beta dx) ) )^2 + a^2 dt^2/dx^2 \sin^2(\beta dx )
1 > 1 + 2 a dt/dx (1 - \cos ( \beta dx ) ) + a^2 dt^2 / dx^2 ( ( 1 - \cos ( \beta dx ) )^2 + \sin^2 (\beta dx) )
0 > 2 (1 - \cos ( \beta dx ) ) + 2 a dt / dx ( 1 + \cos ( \beta dx) )  
dt < - 1/a dx

Accuracy

Taylor:

du(t + dt, x) = u(t, x) + partial u/ partial t dt + 1/2 partial^2 u +partial dt^2 u dt^2 + O(dt^3)

u(t,x) + a dt/dx ( u(t,x) - u(t,x-dx) ) + e = u(t, x) + partial u/ partial t dt + 1/2 partial^2 u +partial dt^2 u dt^2 + O(dt^3)
a dt/dx ( u(t,x) - u(t,x-dx) ) + e = a partial u/ partial x dt + 1/2 partial^2 u +partial dt^2 u dt^2 + O(dt^3)
a dt/dx ( u(t,x) - u(t,x-dx) ) + e = a dt ( (u(t,x) - u(t,x-dx) )/dx - 1/2 partial^2 u / partial x^2 dx + O(dx^2)) + 1/2 partial^2 u / partial dt^2 u dt^2 + O(dt^3)
e = - 1/2 a dt dx 1/2 d^2u/dx^2 + 1/2 partial^2 u / partial dt^2 dt^2 + O(dt dx^2 + dt^3)


